not compiling, but monad stuff is better

src/coq/Utils/MapMonadExtra.v
@@ -25,14 +25,41 @@ Import MonadNotation.
 Import ListNotations.
 
 Open Scope monad.
+Open Scope monad_scope.
+
+Section MonadContext.
+  Context (M : Type -> Type).
+  Context {HM: Monad M}.
+  Context {EQM : Monad.Eq1 M}.
+  Context {EE : Eq1Equivalence M}.  
+  Context {LAWS : @Monad.MonadLawsE M EQM HM}.
+  Context {MRET : @MonadReturns M HM EQM}.
+  Context {MRETSTR : @MonadReturnsStrongBindInv M HM EQM MRET}.
+  Context {EQRET : @Eq1_ret_inv M EQM HM}.
+
+  Existing Instance EQM.
+  Existing Instance LAWS.
 
 
+Lemma map_monad_unfold :
+  forall {A B : Type} (x : A) (xs : list A)
+    (f : A -> M B),
+    map_monad f (x :: xs) =
+    b <- f x;;
+    bs <- map_monad (fun (x0 : A) => f x0) xs;;
+    ret (b :: bs).
+Proof.
+  intros A B x xs f.
+  induction xs; cbn; auto.
+Qed.
+
+  
 Lemma map_monad_length :
-  forall {A B M} `{HM: Monad M} `{EQM : Monad.Eq1 M} `{LAWS : @Monad.MonadLawsE M EQM HM} `{MRET : @MonadReturns M HM EQM} `{MRETSTR : @MonadReturnsStrongBindInv M HM EQM MRET} `{EQRET : @Eq1_ret_inv M EQM HM} (xs : list A) (f : A -> M B) res,
+  forall {A B}  (xs : list A) (f : A -> M B) res,
     MReturns res (map_monad f xs) ->
     length xs = length res.
 Proof.
-  intros A B M HM EQ LAWS MRET MRETSTR EQRET xs.
+  intros A B xs.
   induction xs; intros f res Hmap.
   - cbn in Hmap.
     apply MReturns_ret_inv in Hmap; subst; auto.
@@ -51,6 +78,8 @@ Proof.
     cbn.
     lia.
 Qed.
+
+
 
 (* TODO: can I generalize this? *)
 Lemma map_monad_err_In :
@@ -166,3 +195,200 @@ Proof.
     cbn.
     reflexivity.
 Qed.
+
+Lemma map_monad_map :
+  forall A B C 
+    (f : B -> M C)
+    (g : A -> B)
+    (xs : list A),
+    (map_monad f (map g xs)) ≈ (map_monad (fun x => f ( g x) ) xs).
+Proof.
+  intros. induction xs.
+  - simpl. reflexivity.
+  - simpl. 
+    setoid_rewrite IHxs.
+    reflexivity.
+Qed.
+
+
+Lemma bind_helper :
+  forall A B (m : M A) (f : A -> M B), 
+    (bind m f) ≈ ((bind (bind m ret) f)).
+Proof.
+  intros.
+  rewrite bind_ret_r.
+  reflexivity.
+Qed.
+
+
+
+Lemma bind_f_assoc :
+  forall A B C (a: A) (f : A -> M B) (g : B -> C),
+    eq1 (bind (f a) (fun y => ret (g y)))
+        (bind (bind (f a) ret) (fun y => ret (g y))).
+Proof.
+  intros. rewrite bind_bind. setoid_rewrite bind_ret_l.
+  reflexivity.
+Qed.
+
+
+
+(* more general form of the two above; do we need those two? *) 
+Lemma map_monad_g :
+  forall A B C (f : A -> M B) (g : list B -> C) (xs:list A) (zs : list B)
+    (EQ2 : (bind (map_monad f xs) (fun ys => ret ys)) ≈ (ret (zs))),
+    (bind (map_monad f xs) (fun ys => ret (g ys))) ≈ (ret (g zs)).
+Proof.
+  intros.
+  rewrite bind_helper.
+  rewrite EQ2.
+  rewrite bind_ret_l.
+  reflexivity.
+Qed.
+
+
+Lemma map_monad_cons_ret :
+  forall A B (f : A -> M B) (a:A) (xs:list A) (z : B) (zs : list B)
+    (EQ2 : (bind (map_monad f xs) (fun ys => ret ys)) ≈  (ret (zs))),
+    (bind (map_monad f xs) (fun ys => ret (z::ys))) ≈ (ret ((z::zs))).
+Proof.
+  intros.
+  apply map_monad_g with (g := (fun ys => z::ys)).
+  assumption.
+Qed.
+
+Lemma map_monad_append_ret :
+  forall A B (f : A -> M B) (xs:list A) (ws : list B) (zs : list B)
+    (EQ2 : eq1 (bind (map_monad f xs) (fun ys => ret ys))
+               (ret (zs))),
+    (bind (map_monad f xs) (fun ys => ret (ws ++ ys)%list))
+      ≈
+      (ret ((ws ++ zs)%list)).
+Proof.
+  intros.
+  apply map_monad_g with (g := (fun ys => ws ++ ys)).
+  assumption.
+Qed.
+
+
+Lemma map_monad_app
+      {A B} (f:A -> M B) (l0 l1:list A):
+  map_monad f (l0++l1) ≈
+  bs1 <- map_monad f l0;;
+  bs2 <- map_monad f l1;;
+  ret (bs1 ++ bs2).
+Proof.
+  induction l0 as [| a l0 IH]; simpl; intros.
+  - cbn; rewrite bind_ret_l, bind_ret_r.
+    reflexivity.
+  - cbn.
+    setoid_rewrite IH.
+    repeat setoid_rewrite bind_bind.
+    setoid_rewrite bind_ret_l.
+    reflexivity.
+Qed.
+
+
+
+(* FIXME TODO: This is poorly named and doesn't make sense as a lemma. *)
+Lemma map_monad_In {A B} (l : list A) (f: forall (x : A), In x l -> M B) : M (list B).
+Proof.
+  induction l.
+  - exact (ret []).
+  - refine (b <- f a _;; bs <- IHl _;; ret (b::bs)).
+    + cbn; auto.
+    + intros x Hin.
+      apply (f x).
+      cbn; auto.
+Defined.
+
+(* FIXME TODO: This is poorly named and doesn't make sense as a lemma. *)
+Lemma map_monad_In_unfold :
+  forall {A B} (x : A) (xs : list A) (f : forall (elt:A), In elt (x::xs) -> M B),
+    map_monad_In (x::xs) f = b <- f x (or_introl eq_refl);;
+                            bs <- map_monad_In xs (fun x HIn => f x (or_intror HIn));;
+                            ret (b :: bs).
+Proof.
+  intros A B x xs f.
+  induction xs; cbn; auto.
+Qed.
+
+Definition commutative_maps {A} (g : A -> M A) (f : A -> M A) :=
+    forall x, (y <- g x ;; f y)  ≈ (y <- f x ;; g y).
+  
+Lemma map_monad_commutative_maps :
+  forall A (xs : list A) (g : A -> M A) (f : A -> M A)
+    (HC : commutative_maps g f),
+    (ys <- map_monad g xs ;; map_monad f ys)
+      ≈
+    map_monad (fun x => y <- (g x) ;; f y) xs.
+Proof.
+  (* Is this true? *)
+  
+Admitted.  
+
+
+Check @map_monad.
+
+
+Lemma map_monad_cons
+      {A B} (f:A -> M B) (x:A) (l:list A) :
+  (map_monad f (x::l)) ≈
+  b <- f x;;
+  bs2 <- map_monad f l;;
+  ret (b :: bs2).
+Proof.
+  (* TODO - easy? *)
+Admitted.
+
+Lemma map_monad_nil 
+      {A B} (f:A -> M B) :
+  (map_monad f []) ≈ ret [].
+Proof.
+  (* TODO - very easy *)
+Admitted.  
+
+Lemma sequence : forall {A} (l : list A),
+      sequence (map ret l) ≈ ret l.
+Proof.
+Admitted.  
+
+Lemma map_monad_ret_l : forall {A} (l : list A),
+    map_monad ret l ≈ ret l.
+Proof.
+Admitted.  
+
+Lemma map_monad_ret_nil_inv :
+  forall {A B} (f : A -> M B) (l : list A)
+  (HRet : MReturns [] (map_monad f l)),
+  l = [].
+Proof.
+Admitted.  
+
+Lemma map_monad_ret_nil_inv_pure :
+  forall {A B} (f : A -> M B) (l : list A)
+  (HEq : map_monad f l ≈ ret []),
+  l = [].
+Proof.
+  (* Provable using MReturns_ret_inv and [map_monad_ret_nil_inv] *)
+Admitted.  
+
+Lemma map_monad_In_inv_pure :
+  forall {A B} (f : A -> M B) (x : A) (y : B) (l1 : list A) (l2 : list B)
+    (HIn: In y l2)
+    (HEq: map_monad f l1 ≈ ret l2),
+    exists x, In x l1 /\ f x ≈ ret y.
+Proof.
+Admitted.
+
+Lemma map_monad_In_inv :
+  forall {A B} (f : A -> M B) (x : A) (y : B) (l1 : list A) (l2 : list B)
+    (HIn: In y l2)
+    (HEq: MReturns l2 (map_monad f l1)),
+    exists x, In x l1 /\ (MReturns y (f x)).
+Proof.
+Admitted.
+
+
+
+End MonadContext.
